Hungarian_Method/Hungarian_Method_Instantiation.thy
@@ -1,0 +1,534 @@
+theory Hungarian_Method_Instantiation
+  imports  Primal_Dual_Path_Search Alternating_Forest_Executable Ordered_Map_Heap
+Naive_Primal_Dual "HOL-Library.Rewrite"
+Matching_Augmentation_Executable
+Hungarian_Method_Top_Loop
+begin
+
+text \<open>Let's instantiate the path search\<close>
+
+global_interpretation pd_path_search_spec: primal_dual_path_search_spec
+  (*the graph*)
+  where G = G
+   and left = left
+   and right = right
+   and buddy = buddy
+   and edge_costs = edge_costs
+   and right_neighbs = right_neighbs
+  (*the forest*)
+   and evens = evens
+   and odds = odds
+   and abstract_forest = "abstract_forest parent_lookup"
+   and get_path = "get_path parent_lookup"
+   and extend_forest_even_unclassified = 
+     "extend_forest_even_unclassified parent_upd vset_insert 
+          origin_upd origin_lookup" 
+   and empty_forest = 
+      "empty_forest parent_empty vset_empty to_list origin_empty origin_upd"
+  (*the heap*)
+   and heap_insert = queue_insert
+   and heap_decrease_key = queue_decrease_key
+   and heap_empty = queue_empty
+   and heap_extract_min = queue_extract_min
+  (*the potential*)
+   and initial_pot = initial_pot
+   and potential_lookup = potential_lookup
+   and potential_upd = potential_upd
+  (*missed change in potential*)
+   and missed_lookup = missed_lookup
+   and missed_empty = missed_empty
+   and missed_upd = missed_upd
+  (*best even neighbour map*)
+   and ben_upd = ben_upd
+   and ben_lookup = ben_lookup
+   and ben_empty = ben_empty
+  (*sets of vertices*)
+   and vset_isin= vset_isin
+   and to_list = to_list
+   and vset_to_set = vset_to_set
+   and vset_insert = vset_insert
+   and vset_empty = vset_empty
+ for (*the graph*) G left right buddy edge_costs right_neighbs
+     (*the forest*) parent_lookup  parent_upd parent_empty
+                    origin_upd origin_lookup origin_empty 
+     (*the potential*) initial_pot potential_lookup potential_upd
+     (*missed change in potential*) missed_lookup missed_empty missed_upd
+     (*best even neighbour map*) ben_upd ben_lookup ben_empty
+     (*sets of vertices*) vset_isin to_list vset_to_set vset_insert vset_empty
+
+defines search_path = pd_path_search_spec.search_path
+  and search_path_loop_impl = pd_path_search_spec.search_path_loop_impl
+  and new_potential = pd_path_search_spec.new_potential
+  and w\<^sub>\<pi>=pd_path_search_spec.w\<^sub>\<pi>
+  and path_search_initial_state = pd_path_search_spec.initial_state
+  and unmatched_lefts= pd_path_search_spec.unmatched_lefts
+  and init_best_even_neighbour = pd_path_search_spec.init_best_even_neighbour
+  and update_best_even_neighbours = pd_path_search_spec.update_best_even_neighbours
+  and update_best_even_neighbour = pd_path_search_spec.update_best_even_neighbour
+  and path_search_forest_roots = pd_path_search_spec.forest_roots
+  done
+
+(*manual fix of "partially applied constant on left hand side of equation"*)
+lemmas [code] = pd_path_search_spec.search_path_def[folded search_path_def]
+                pd_path_search_spec.initial_state_def[folded path_search_initial_state_def]
+                
+locale path_search_instantiated_correct = 
+  fixes G::"('v::linorder) set set"
+    and edge_costs::"'v \<Rightarrow> 'v \<Rightarrow> real"
+    and left::'vset
+    and right::'vset
+    and in_G::"'v \<Rightarrow> 'v \<Rightarrow> bool"
+    and right_neighbs::"'v \<Rightarrow> 'vset"
+
+    and buddy::"'v \<Rightarrow> 'v option"
+
+   and potential_upd::"'potential \<Rightarrow> 'v \<Rightarrow> real \<Rightarrow> 'potential"
+   and potential_lookup::"'potential \<Rightarrow> 'v \<Rightarrow> real option"
+   and potential_invar::"'potential \<Rightarrow> bool"
+   and initial_pot::"'potential"
+
+   and ben_empty::'ben
+   and ben_lookup::"'ben \<Rightarrow> 'v \<Rightarrow> 'v option"
+   and ben_upd::"'ben \<Rightarrow> 'v \<Rightarrow> 'v \<Rightarrow> 'ben"
+   and ben_invar::"'ben \<Rightarrow> bool"
+
+   and missed_empty::'miss
+   and missed_lookup::"'miss \<Rightarrow> 'v \<Rightarrow> real option"
+   and missed_upd::"'miss \<Rightarrow> 'v \<Rightarrow> real \<Rightarrow> 'miss"
+   and missed_invar::"'miss \<Rightarrow> bool"
+
+   and to_list::"'vset \<Rightarrow> 'v list"
+   and vset_to_set::"'vset \<Rightarrow> 'v set"
+   and vset_isin::"'v \<Rightarrow> 'vset \<Rightarrow> bool"
+   and vset_empty::"'vset"
+   and vset_insert::"'v \<Rightarrow> 'vset \<Rightarrow> 'vset"
+   and vset_invar::"'vset \<Rightarrow> bool"
+
+   and parent_empty::'parent
+    and   parent_upd::"'v\<Rightarrow>'v\<Rightarrow>'parent\<Rightarrow>'parent"
+    and   parent_lookup::"'parent \<Rightarrow> 'v \<Rightarrow> 'v option"
+    and   parent_delete::"'v \<Rightarrow> 'parent \<Rightarrow>'parent"
+    and   parent_invar::"'parent \<Rightarrow> bool"
+
+and   origin_empty::'origin
+and   origin_upd::"'v\<Rightarrow>'v\<Rightarrow>'origin\<Rightarrow>'origin"
+and   origin_lookup::"'origin \<Rightarrow> 'v \<Rightarrow> 'v option"
+and   origin_invar::"'origin \<Rightarrow> bool"
+assumes G: "bipartite G (vset_to_set left) (vset_to_set right)"
+           "\<And> u v. in_G u v \<longleftrightarrow> {u, v} \<in> G"
+           "vset_invar left" "vset_invar right"
+
+           "\<And> v. v \<in> vset_to_set left \<Longrightarrow> vset_invar (right_neighbs v)"
+           "\<And> v. v \<in> vset_to_set left \<Longrightarrow> vset_to_set (right_neighbs v) = {u | u. {v, u} \<in> G}"
+           "\<And> u v. {u, v} \<in> G \<Longrightarrow> edge_costs u v = edge_costs v u"
+           "\<And> u v. {u, v} \<in> G \<Longrightarrow> abstract_real_map (potential_lookup initial_pot) u 
+                                 + abstract_real_map (potential_lookup initial_pot) v 
+                                  \<le> edge_costs u v"
+  
+and matching: "\<And> u v. buddy u = Some v \<Longrightarrow> buddy v = Some u"
+              "graph_matching G {{u, v} | u v. buddy u = Some v}"
+              "\<And> u v. {u, v} \<in> {{u, v} | u v. buddy u = Some v} 
+           \<Longrightarrow> abstract_real_map (potential_lookup initial_pot) u 
+                                 + abstract_real_map (potential_lookup initial_pot) v 
+                                  = edge_costs u v"
+and potential:
+ "potential_invar initial_pot"
+ "\<And> pot x s. potential_invar pot \<Longrightarrow> potential_invar (potential_upd pot x s)"
+ "\<And> pot x s. potential_invar pot \<Longrightarrow> potential_lookup (potential_upd pot x s) =
+                (potential_lookup pot)(x \<mapsto> s)"
+and best_even_neighbour:
+ "ben_invar ben_empty"
+  "\<And> ben x s. ben_invar ben \<Longrightarrow> ben_invar (ben_upd ben x s)"
+  "\<And> ben x s. ben_invar ben \<Longrightarrow> ben_lookup (ben_upd ben x s) =
+                (ben_lookup ben)(x \<mapsto> s)"
+  "\<And> x. ben_lookup ben_empty x = None"
+and vset:
+ "vset_invar vset_empty" "vset_to_set vset_empty = {}"
+ "\<And> V v. vset_invar V \<Longrightarrow> vset_invar (vset_insert v V)"
+ "\<And> V v. vset_invar V \<Longrightarrow> vset_to_set (vset_insert v V) = insert v (vset_to_set V)"
+ "\<And> V v. vset_invar V \<Longrightarrow> vset_isin v V \<longleftrightarrow> v \<in> vset_to_set V"
+ "\<And> V vs. \<lbrakk>vset_invar V; to_list V = vs\<rbrakk> \<Longrightarrow> distinct vs"
+ "\<And> V vs. \<lbrakk>vset_invar V; to_list V = vs\<rbrakk> \<Longrightarrow> set vs = vset_to_set V"
+and missed:
+ "missed_invar missed_empty" "\<And> x. missed_lookup missed_empty x= None"
+  "\<And> missed x s. missed_invar missed \<Longrightarrow> missed_invar (missed_upd missed x s)"
+  "\<And> missed x s. missed_invar missed \<Longrightarrow> missed_lookup (missed_upd missed x s) =
+                (missed_lookup missed)(x \<mapsto> s)"
+  "\<And> x. missed_lookup missed_empty x = None"
+and potential_in_G:
+"dom (potential_lookup initial_pot) \<subseteq> vset_to_set left \<union> vset_to_set right"
+    and parent:
+    "parent_invar parent_empty"
+    "parent_lookup parent_empty = (\<lambda> x. None)"
+    "\<And> par x s. parent_invar par \<Longrightarrow> parent_invar (parent_upd x s par)"
+    "\<And> par x s. parent_invar par \<Longrightarrow> parent_lookup (parent_upd x s par) =
+                (parent_lookup par)(x \<mapsto> s)"
+    and origin:
+    "origin_invar origin_empty"
+    "origin_lookup origin_empty = (\<lambda> x. None)"
+    "\<And> par x s. origin_invar par \<Longrightarrow> origin_invar (origin_upd x s par)"
+    "\<And> par x s. origin_invar par \<Longrightarrow> origin_lookup (origin_upd x s par) =
+                (origin_lookup par)(x \<mapsto> s)"
+begin
+
+interpretation fmnlp: forest_manipulation
+  where vset_flatten = to_list
+  using vset(1-5) vset (6-7)[OF _ refl]
+  by(auto intro!: forest_manipulation.intro parent origin)
+
+abbreviation "forest_invar == fmnlp.forest_invar"
+
+interpretation  satisfied_simple:
+ alternating_forest_spec evens odds "get_path parent_lookup" "abstract_forest parent_lookup"
+     forest_invar roots vset_invar vset_to_set
+  unfolding abstract_forest_def get_path_def
+  apply(intro alternating_forest_spec.intro 
+      fmnlp.simple_invariant_consequences)
+  using fmnlp.complex_invariant_consequences(1,2) 
+  by(auto simp add: fmnlp.get_path_correct(1,2,3,4,5))
+
+interpretation fe_spec: 
+     alternating_forest_ordinary_extension_spec vset_invar vset_to_set evens odds
+     "get_path parent_lookup" "abstract_forest parent_lookup" forest_invar roots vset_empty
+     "extend_forest_even_unclassified parent_upd vset_insert origin_upd origin_lookup"
+     "empty_forest parent_empty vset_empty to_list origin_empty origin_upd"
+  apply(intro alternating_forest_ordinary_extension_spec.intro
+      satisfied_simple.alternating_forest_spec_axioms
+      alternating_forest_ordinary_extension_spec_axioms.intro)
+  by (simp_all add:  fmnlp.extension_main_preservation fmnlp.satisfied_simple_extension_precond_same
+      fmnlp.extension_abstract_is fmnlp.extension_evens fmnlp.extension_odds fmnlp.extension_roots 
+      fmnlp.empty_forest_correctess  extend_forest_even_unclassified_def 
+      abstract_forest_def empty_forest_def )
+
+interpretation pd_path_search: primal_dual_path_search
+  (*the graph*)
+  where G = G
+   and left = left
+   and right = right
+   and buddy = buddy
+   and edge_costs = edge_costs
+   and right_neighbs = right_neighbs
+  (*the forest*)
+   and evens = evens
+   and odds = odds
+   and abstract_forest = "abstract_forest parent_lookup"
+   and get_path = "get_path parent_lookup"
+   and extend_forest_even_unclassified = 
+     "extend_forest_even_unclassified parent_upd vset_insert 
+          origin_upd origin_lookup" 
+   and empty_forest = 
+      "empty_forest parent_empty vset_empty to_list origin_empty origin_upd"
+   and roots = roots
+   and forest_invar = forest_invar
+  (*the heap*)
+   and heap_insert = queue_insert
+   and heap_decrease_key = queue_decrease_key
+   and heap_empty = queue_empty
+   and heap_extract_min = queue_extract_min
+   and heap_invar = queue_invar
+   and heap_abstract = queue_abstract
+  (*the potential*)
+   and initial_pot = initial_pot
+   and potential_lookup = potential_lookup
+   and potential_upd = potential_upd
+  (*missed change in potential*)
+   and missed_lookup = missed_lookup
+   and missed_empty = missed_empty
+   and missed_upd = missed_upd
+  (*best even neighbour map*)
+   and ben_upd = ben_upd
+   and ben_lookup = ben_lookup
+   and ben_empty = ben_empty
+  (*sets of vertices*)
+   and vset_isin= vset_isin
+   and to_list = to_list
+   and vset_to_set = vset_to_set
+   and vset_insert = vset_insert
+   and vset_empty = vset_empty
+proof(rule primal_dual_path_search.intro, goal_cases)
+  case 1
+  thus ?case
+    using fe_spec.alternating_forest_ordinary_extension_spec_axioms
+    by simp
+next
+  case 2
+  thus ?case
+    using key_value_queue_spec_satisfied.key_value_queue_axioms by simp
+next
+  case 3
+  thus ?case
+    apply(intro primal_dual_path_search_axioms.intro G potential 
+            best_even_neighbour vset(1-5) missed  potential_in_G)+
+    using matching(2) vset(7)
+    by (fastforce intro: matching(1,3) vset(6)
+               simp add: pd_path_search_spec.\<M>_def) +   
+qed
+
+lemmas search_path_correct = pd_path_search.search_path_correct
+end
+
+locale build_init_potential_spec =
+  fixes vs::"'v list"
+  and   neighbs::"'v \<Rightarrow> 'vset option"
+  and   to_list::"'vset \<Rightarrow> 'v list"
+  and   vset_to_set::"'vset \<Rightarrow> 'v set"
+  and   vset_invar::"'vset \<Rightarrow> bool"
+  and   edge_costs::"'v \<Rightarrow> 'v \<Rightarrow> real"
+  and   empty_potential::'potential
+  and   potential_upd::"'potential \<Rightarrow> 'v \<Rightarrow> real  \<Rightarrow> 'potential"
+  and   potential_lookup::"'potential \<Rightarrow> 'v \<Rightarrow> real option"
+  and   potential_invar::"'potential \<Rightarrow> bool"
+begin
+
+definition "init_potential = 
+  foldl (\<lambda> \<pi> u. case neighbs u of None \<Rightarrow> \<pi>
+                | Some nbs \<Rightarrow>
+             foldl (\<lambda> \<pi> v. (case potential_lookup \<pi> u of
+                               None \<Rightarrow> potential_upd  \<pi> u (edge_costs u v)
+                              | Some r \<Rightarrow> if r \<le> edge_costs u v then \<pi>
+                                          else potential_upd  \<pi> u (edge_costs u v)))
+                  \<pi> (to_list nbs))
+        empty_potential vs"
+
+lemmas [code] = init_potential_def
+end
+
+global_interpretation build_init_pot: build_init_potential_spec
+  where potential_lookup = potential_lookup 
+and potential_upd = potential_upd
+and empty_potential = empty_potential
+and edge_costs = edge_costs
+and to_list = to_list 
+and neighbs = neighbs 
+and vs = vs
+for potential_lookup potential_upd empty_potential
+    edge_costs to_list neighbs vs
+  defines init_potential = build_init_pot.init_potential
+  done
+
+locale build_init_potential = 
+build_init_potential_spec+
+assumes vs_distinct: "distinct vs"
+and neighbs: "\<And> v N. neighbs v = Some N \<Longrightarrow> vset_invar N"
+and vset: "\<And> S. vset_invar S \<Longrightarrow> distinct (to_list S)"
+          "\<And> S. vset_invar S \<Longrightarrow> vset_to_set S = set (to_list S)"
+and potential:
+     "potential_invar empty_potential"
+     "potential_lookup empty_potential = (\<lambda> v. None)"
+     "\<And> p v r. potential_invar p \<Longrightarrow> potential_invar (potential_upd p v r)"
+     "\<And> p v r. potential_invar p \<Longrightarrow>
+        potential_lookup (potential_upd p v r) = (potential_lookup p)(v \<mapsto> r)"
+begin
+
+definition "less_than_edgs_bet p E = 
+           (\<forall> e \<in> E. p (fst e) \<le> edge_costs (fst e) (snd e))" 
+
+
+lemma less_than_edgs_bet_empty: "less_than_edgs_bet p {}"
+  by(auto simp add: less_than_edgs_bet_def)
+
+lemma init_potential_props:
+   "potential_invar init_potential"
+   "\<And> u v N. \<lbrakk>u \<in> set vs; neighbs u = Some N; v \<in> vset_to_set N\<rbrakk> \<Longrightarrow>
+            abstract_real_map (potential_lookup init_potential) u \<le> edge_costs u v"
+   "dom (potential_lookup init_potential) = 
+    { v| v x. v \<in> set vs \<and> neighbs v \<noteq> None \<and>
+           vset_to_set (the (neighbs v)) \<noteq> {}}"
+proof-
+  define inner_f where "inner_f = (\<lambda> u \<pi> v. (case potential_lookup \<pi> u of
+                               None \<Rightarrow> potential_upd  \<pi> u (edge_costs u v)
+                              | Some r \<Rightarrow> if r \<le> edge_costs u v then \<pi>
+                                          else potential_upd  \<pi> u (edge_costs u v)))"
+  define outer_f where "outer_f = (\<lambda> \<pi> u. case neighbs u of None \<Rightarrow> \<pi>
+                | Some nbs \<Rightarrow> foldl (inner_f u) \<pi> (to_list nbs))"
+  have inner_f_invar_pres: "potential_invar \<pi> \<Longrightarrow> potential_invar (inner_f u \<pi> v)" for u \<pi> v
+    by(auto simp add: inner_f_def potential(3) split: option.split)
+  have inner_f_prop_pres: 
+   "less_than_edgs_bet (abstract_real_map (potential_lookup (inner_f u \<pi> v)))
+           (insert (u, v) E)"
+    "fst ` (insert (u, v) E) = dom (potential_lookup (inner_f u \<pi> v))"
+   if "less_than_edgs_bet (abstract_real_map (potential_lookup \<pi>)) E" 
+      "potential_invar \<pi>" 
+      "fst ` E = dom (potential_lookup \<pi>)"for E \<pi> u v
+    using  that 
+      by(auto simp add: inner_f_def less_than_edgs_bet_def abstract_real_map_def
+           potential(4) split: option.split)
+    have inner_fold_invar_pres:
+     "potential_invar (foldl (inner_f u) \<pi> xs)"
+     if "potential_invar \<pi>" for u \<pi> xs
+    proof-
+      define ys where "ys = rev xs"
+      show ?thesis
+        using that
+      unfolding foldl_conv_foldr ys_def[symmetric]
+      by(induction ys)
+        (auto intro!: inner_f_invar_pres)
+  qed
+  have inner_fold_props_pres:
+      "less_than_edgs_bet (abstract_real_map (potential_lookup (foldl (inner_f u) \<pi> xs)))
+           (E \<union> {(u, v) | v. v \<in> set xs})" (is ?rslt1)
+    "fst `  (E \<union> {(u, v) | v. v \<in> set xs}) = dom (potential_lookup (foldl (inner_f u) \<pi> xs))" (is ?rslt2)
+    if "less_than_edgs_bet (abstract_real_map (potential_lookup \<pi>)) E" 
+      "potential_invar \<pi>" 
+      "fst ` E = dom (potential_lookup \<pi>)"
+    for u \<pi> xs E
+  proof-
+      define ys where "ys = rev xs"
+      have  "?rslt1 \<and>?rslt2"
+        using that 
+        unfolding foldl_conv_foldr ys_def[symmetric] set_rev[of xs, symmetric]
+      proof(induction ys)
+        case Nil
+        then show ?case by auto
+      next
+        case (Cons y ys)
+        note IH_applied = conjunct1[OF Cons(1)[OF Cons(2,3,4)]] 
+                          conjunct2[OF Cons(1)[OF Cons(2,3,4)]]
+        note potential_now = inner_fold_invar_pres[OF Cons(3), of u "rev ys",
+                                simplified foldl_conv_foldr rev_rev_ident]
+        note inner_f_props_applied = inner_f_prop_pres[OF 
+                      IH_applied(1) potential_now IH_applied(2)] 
+
+        show ?case 
+        proof(rule, goal_cases)
+          case 1
+          show ?case
+            apply (subst foldr_Cons o_apply)+
+            apply(rule rev_iffD2[OF inner_f_props_applied(1)[of u y]])
+            apply(rule arg_cong[of "_ ::_ set"])
+            by auto
+        next
+          case 2
+           show ?case
+            apply (subst foldr_Cons o_apply inner_f_props_applied(2)[symmetric])+         
+             by force
+         qed
+       qed
+       thus ?rslt1 ?rslt2 
+         by auto
+     qed
+     let ?new_es = "{(u, v) | u v. u \<in> set vs \<and> neighbs u \<noteq> None \<and> v \<in> vset_to_set (the (neighbs u))}"
+     have outer_iteration_pres:
+      "potential_invar (foldl outer_f \<pi> vs)" (is ?rslt0)
+      "less_than_edgs_bet (abstract_real_map (potential_lookup (foldl outer_f \<pi> vs)))
+           (E \<union> ?new_es)" (is ?rslt1)
+    "fst `  (E \<union> ?new_es) = dom (potential_lookup (foldl outer_f \<pi> vs))" (is ?rslt2)
+    if "less_than_edgs_bet (abstract_real_map (potential_lookup \<pi>)) E" 
+      "potential_invar \<pi>" 
+      "fst ` E = dom (potential_lookup \<pi>)"
+    for \<pi> E 
+     proof-
+       define vvs where "vvs = rev vs"
+       have "?rslt0 \<and> ?rslt1 \<and> ?rslt2"
+         using that
+         unfolding foldl_conv_foldr vvs_def[symmetric] set_rev[of vs, symmetric]
+       proof(induction vvs)
+         case Nil
+         then show ?case by auto
+       next
+         case (Cons u vvs)
+         note IH_applied_all = Cons(1)[OF Cons(2,3,4)]
+         note IH_applied = conjunct1[OF IH_applied_all]
+                           conjunct1[OF conjunct2[OF IH_applied_all]]
+                           conjunct2[OF conjunct2[OF IH_applied_all]]
+         show ?case
+           apply(subst foldr_Cons o_apply)+ 
+           apply(subst outer_f_def, subst (3) outer_f_def, subst (5) outer_f_def)
+         proof(cases "neighbs u", goal_cases)
+           case 1
+           note one = this
+           show ?case 
+             apply(subst 1 option.case(1))+
+           proof(rule conjI[OF IH_applied(1)], rule, goal_cases)
+             case 1
+             show ?case
+               apply(rule rev_iffD2[OF IH_applied(2)])
+               apply(rule arg_cong[of "_ ::_ set"])
+               using one by auto
+           next
+             case 2
+             show ?case
+               using one
+               by(subst IH_applied(3)[symmetric]) auto
+           qed
+         next
+           case (2 N)
+           note two = this
+           have vset_invar_N:"vset_invar N"
+             using "2" neighbs by auto
+           show ?case 
+             apply(subst 2 option.cases(2))+
+             proof(rule, goal_cases)
+             case 1
+             show ?case
+               apply(rule rev_iffD2[OF inner_fold_invar_pres[OF IH_applied(1)]])
+               by auto
+           next
+             case 2
+             show ?case
+             proof(rule, goal_cases)
+               case 1
+               show ?case
+                 apply(rule rev_iffD2[OF inner_fold_props_pres(1)[OF 
+                           IH_applied(2,1,3), of u "to_list (the (neighbs u))"]])
+                 apply(subst two option.sel)+
+                 apply(rule arg_cong[of "_ ::_ set"])
+                 using two vset(2)[OF  vset_invar_N] 
+                 by auto
+             next 
+               case 2
+               show ?case
+                 apply(subst inner_fold_props_pres(2)[OF IH_applied(2,1,3),
+ of u "to_list (the (neighbs u))", symmetric, simplified  
+        two  option.sel vset(2)[OF vset_invar_N]])
+                 using two vset(2)[OF  vset_invar_N] 
+                 by auto
+             qed
+           qed
+         qed
+       qed
+    
+       thus ?rslt0 ?rslt1 ?rslt2 
+         by auto
+     qed
+     note final_props =  outer_iteration_pres[OF less_than_edgs_bet_empty potential(1),
+                simplified potential(2), simplified]
+     have init_pot_is: "init_potential = foldl outer_f empty_potential vs"
+       by(subst init_potential_def outer_f_def inner_f_def)+ simp
+     show  "potential_invar init_potential"
+   "\<And> u v N. \<lbrakk>u \<in> set vs; neighbs u = Some N; v \<in> vset_to_set N\<rbrakk> \<Longrightarrow>
+            abstract_real_map (potential_lookup init_potential) u \<le> edge_costs u v"
+      "dom (potential_lookup init_potential) = 
+      { v | v x. v \<in> set vs \<and> neighbs v \<noteq> None \<and>
+           vset_to_set (the (neighbs v)) \<noteq> {}}"
+       using final_props(1,2)
+       by(force simp add: init_pot_is final_props(3)[symmetric]
+                          less_than_edgs_bet_def)+
+   qed
+end
+
+hide_const left
+
+thm search_path_def
+global_interpretation hungarian:
+hungarian_loop_spec
+where path_search = "\<lambda> M P. search_path left (\<lambda> M. buddy_lookup M)
+                    (edge_costs::('a::linorder) \<Rightarrow> 'a \<Rightarrow> real) right_neighbs parent_lookup
+                     parent_upd parent_empty  origin_upd origin_lookup origin_empty P 
+                     potential_lookup potential_upd missed_lookup  missed_empty missed_upd 
+                     ben_upd ben_lookup ben_empty to_list vset_insert vset_empty"
+and edge_costs = "(\<lambda> e. edge_costs (pick_one e) (pick_another e))"
+and init_potential = "init_potential potential_lookup potential_upd
+                          empty_potential edge_costs to_list neighbs vs"
+and potential_abstract = "(\<lambda> \<pi> v. abstract_real_map (potential_lookup \<pi>) v)"
+for 
+     (*the graph*) G left right buddy edge_costs right_neighbs
+     (*the forest*) parent_lookup  parent_upd parent_empty
+                    origin_upd origin_lookup origin_empty 
+     (*the potential*) initial_pot potential_lookup potential_upd
+     (*missed change in potential*) missed_lookup missed_empty missed_upd
+     (*best even neighbour map*) ben_upd ben_lookup ben_empty
+     (*sets of vertices*) vset_isin to_list vset_to_set vset_insert vset_empty
+  done
+
+end
