Hungarian_Method/Hungarian_Method_Top_Loop.thy
@@ -1,0 +1,760 @@
+theory Hungarian_Method_Top_Loop
+  imports Primal_Dual_Bipartite_Matching.Matching_LP
+          Path_Search_Result Matching_Augmentation_Executable
+begin
+
+lemma bipartite_same_matcheds_on_both_sides:
+  assumes "bipartite G L R" "graph_matching G M"
+  shows   "card (Vs M \<inter> L) = card (Vs M \<inter> R)"
+proof-
+  define f where "f = (\<lambda> l. SOME r. \<exists> e \<in> M. {l, r} = e)"
+  have "inj_on f (Vs M \<inter> L)"
+  proof(rule inj_onI, goal_cases)
+    case (1 l l')
+     have "{l, f l} \<in> M"
+      using 1(1) assms(1,2) 
+      by(auto simp add: Vs_def  insert_commute  f_def
+                   elim!: bipartite_edgeE[of _ G L R] 
+                   dest!: set_mp[of M G] dest: someI)
+    moreover have "{l', f l'} \<in> M"
+      using 1(2) assms(1,2) 
+      by(auto simp add: Vs_def  insert_commute  f_def
+                   elim!: bipartite_edgeE[of _ G L R] 
+                   dest!: set_mp[of M G] dest: someI)
+    ultimately show ?case
+      using 1(3)  assms(2) 
+      by(auto intro!: doubleton_in_matching(2))
+  qed
+  moreover have "f ` (Vs M \<inter> L) = Vs M \<inter> R"
+  proof(rule, all \<open>rule\<close>, goal_cases)
+    case (1 r)
+    then obtain l e where le: "l \<in> L" "l \<in> e" "e \<in> M" "r = f l"
+      by(auto simp add: Vs_def)
+    moreover hence lflM:"{l, f l} \<in> M"
+      using assms(1,2) 
+      by(auto simp add: insert_commute  f_def
+                   elim!: bipartite_edgeE[of _ G L R] 
+                   dest!: set_mp[of M G] dest: someI)
+    ultimately have "e = {l, f l}" "f l = r" "r \<in> R"
+      using assms(1,2) matching_unique_match[of M l e "{l, f l}"] 
+      by(auto  elim!: bipartite_edgeE[of _ G L R] dest!: set_mp[of M G] 
+            simp add: doubleton_eq_iff  bipartite_def disjoint_iff)
+    thus ?case 
+      using edges_are_Vs_2[OF lflM] 
+      by auto
+  next
+    case (2 r)
+    then obtain l where l: "{l ,r} \<in> M" 
+      using 2(1) assms(1,2) 
+      by(auto simp add: Vs_def  insert_commute 
+                   elim!: bipartite_edgeE[of _ G L R] 
+                   dest!: set_mp[of M G] )
+    have "f l = r" "l \<in> L"
+      using assms(1,2) l 2 someI[of "\<lambda> r. \<exists> e \<in> M. {l, r} = e", OF bexI, OF refl l]
+       by(auto  elim!: bipartite_edgeE[of _ G L R] dest!: set_mp[of M G]
+                intro: doubleton_in_matching(1)
+             simp add: f_def doubleton_eq_iff bipartite_def disjoint_iff)
+     thus ?case
+       using edges_are_Vs[of l "f l"] l  
+       by auto
+   qed
+  ultimately have "bij_betw f (Vs M \<inter> L) (Vs M \<inter> R)"
+    by(auto simp add: bij_betw_def)
+  thus ?thesis
+    by(rule bij_betw_same_card)
+qed
+
+lemma all_left_matched_perfect:
+  assumes "bipartite G L R"
+          "L \<subseteq> Vs M" "card L = card R"
+          "graph_matching G M" "finite R"
+    shows "perfect_matching G M"
+proof(rule perfect_matchingI, goal_cases)
+  case 1
+  then show ?case 
+    using assms(4) by simp 
+next
+  case 2
+  then show ?case 
+   using assms(4) by simp
+next
+  case 3
+  have "Vs M \<inter> L = L"
+    using assms(1,2,4)
+    by blast
+  hence "card L = card (Vs M \<inter> R)"
+    using bipartite_same_matcheds_on_both_sides[OF assms(1,4)] by simp
+  hence "card (Vs M \<inter> R) = card R"
+    using assms(3) by simp
+  hence "Vs M \<inter> R = R"
+    using assms(5) 
+    by(intro card_subset_eq) auto
+  hence "R \<subseteq> Vs M" 
+    by auto
+  hence "Vs G \<subseteq> Vs M"
+    using assms(2) bipartite_vs_subset[OF assms(1)] by auto
+  then show ?case 
+    by (simp add: assms(4) subgraph_vs_subset_eq)  
+qed
+
+lemma no_perfect_matching_one_side_bigger:
+  assumes "bipartite G L R" "L \<union> R \<subseteq> Vs G" 
+          "card L \<noteq> card R"
+    shows "\<nexists> M. perfect_matching G M"
+proof(rule ccontr, goal_cases)
+  case 1
+  then obtain M where M: "perfect_matching G M" by auto
+  hence "card (Vs M \<inter> L) = card (Vs M \<inter> R)" 
+    using assms(1) bipartite_same_matcheds_on_both_sides perfect_matchingD(1,2) by blast
+  moreover have "card (Vs M \<inter> L) = card L"  "card (Vs M \<inter> R) = card R"
+    using M assms(2) perfect_matchingD(3)
+    by(fastforce intro!: arg_cong[of _ _ card ])+
+  ultimately have "card L = card R" 
+    by simp
+  thus False
+    using assms(3) by simp
+qed
+
+lemma in_symmetric_diff_iff:
+   "x \<in> X \<oplus> Y \<longleftrightarrow> x \<in> X \<and> x \<notin> Y \<or> x \<in> Y \<and> x \<notin> X"
+  by(auto simp add: symmetric_diff_def)
+
+lemma Berge_2':         
+  assumes aug_path: "matching_augmenting_path M p" "M \<subseteq> G" "path G p" "distinct p" and
+    finite: "finite M" and
+    matchings: "graph_matching G M"
+  shows "graph_matching G (M \<oplus> set (edges_of_path p))" 
+  using assms
+  by (auto intro!: Berge_2[of _ _ G] dest: Berge_2(3))
+
+section \<open>Top Loop for Hungarian Method\<close>
+
+no_translations
+  "_Collect p P"      <= "{p. P}"
+  "_Collect p P"      <= "{p|xs. P}"
+  "_CollectIn p A P"  <= "{p : A. P}"
+
+datatype result = success | failure | notyetterm
+
+record ('buddy, 'potential) hungarian_state = 
+     buddies::'buddy
+     potential::'potential
+     result::result
+
+subsection \<open>Locale for Implementation\<close>
+
+locale hungarian_loop_spec =
+fixes potential_abstract::"'potential \<Rightarrow> 'v \<Rightarrow> real"
+   and init_potential::'potential
+   and potential_invar::"'potential \<Rightarrow> bool"
+
+   and empty_matching::'matching
+   and matching_invar::"'matching \<Rightarrow> bool"
+   and augment::"'matching \<Rightarrow> 'v list \<Rightarrow> 'matching"
+   and matching_abstract::"'matching \<Rightarrow> 'v set set"
+
+   and edge_costs::"'v set \<Rightarrow> real"
+
+   and card_L card_R::nat
+   and path_search::"'matching \<Rightarrow> 'potential \<Rightarrow> ('v, 'potential) path_search_result"
+   and G::"'v set set"
+begin
+
+function (domintros) hungarian_loop::
+   "('matching, 'potential) hungarian_state \<Rightarrow> ('matching, 'potential) hungarian_state"
+   where "hungarian_loop state =
+     (let M = buddies state;
+          \<pi> = potential state in
+       case path_search M \<pi> of
+         Dual_Unbounded \<Rightarrow> state \<lparr>result:=failure\<rparr>
+       | Lefts_Matched \<Rightarrow> state \<lparr>result:=success\<rparr>
+       | Next_Iteration P \<pi>' \<Rightarrow>
+         let M' = augment M P
+         in hungarian_loop (state \<lparr>buddies:=M', potential := \<pi>' \<rparr>))"
+  by pat_completeness auto
+
+partial_function (tailrec) hungarian_loop_impl::
+   "('matching, 'potential) hungarian_state \<Rightarrow> ('matching, 'potential) hungarian_state"
+   where "hungarian_loop_impl state =
+     (let M = buddies state;
+          \<pi> = potential state in
+       case path_search M \<pi> of
+         Dual_Unbounded \<Rightarrow> state \<lparr>result:=failure\<rparr>
+       | Lefts_Matched \<Rightarrow> state \<lparr>result:=success\<rparr>
+       | Next_Iteration P \<pi>' \<Rightarrow>
+         let M' = augment M P
+         in hungarian_loop_impl (state \<lparr>buddies:=M', potential := \<pi>' \<rparr>))"
+
+definition "initial_state = \<lparr>buddies = empty_matching, potential = init_potential, result = notyetterm\<rparr>"
+
+definition "hungarian = 
+  (if card_L \<noteq> card_R then None
+   else
+   let final_state = hungarian_loop_impl initial_state
+   in (case result final_state 
+        of failure \<Rightarrow> None
+       | success \<Rightarrow> Some (buddies final_state)))"
+
+lemmas [code] = hungarian_loop_impl.simps initial_state_def hungarian_def
+
+lemma hungarian_loop_impl_same:
+  assumes "hungarian_loop_dom state"
+  shows   "hungarian_loop_impl state = hungarian_loop state"
+  apply(induction rule: hungarian_loop.pinduct[OF assms])
+  apply(subst hungarian_loop_impl.simps)
+  apply(subst hungarian_loop.psimps)
+  by(auto simp add: Let_def split: path_search_result.splits)
+
+definition  "hungarian_loop_upd state =
+     (let M = buddies state;
+          \<pi> = potential state;
+          P = the_path (path_search M \<pi>);
+          \<pi>' = the_pot (path_search M \<pi>); 
+          M' = augment M P
+       in state \<lparr>buddies:=M', potential := \<pi>' \<rparr>)"
+
+definition  "hungarian_loop_fail state = (state \<lparr> result:=failure \<rparr>)"
+definition  "hungarian_loop_succ state = (state \<lparr> result:=success \<rparr>)"
+
+definition  "hungarian_loop_fail_cond state =
+     (let M = buddies state;
+          \<pi> = potential state in
+       case path_search M \<pi> of
+         Dual_Unbounded \<Rightarrow> True
+       | Lefts_Matched \<Rightarrow> False
+       | Next_Iteration P \<pi>' \<Rightarrow> False)"
+
+lemma hungarian_loop_fail_condE:
+"hungarian_loop_fail_cond state \<Longrightarrow>
+(path_search (buddies state) (potential state) = Dual_Unbounded \<Longrightarrow> P)
+ \<Longrightarrow> P"
+and hungarian_loop_fail_condI:
+"path_search (buddies state) (potential state) = Dual_Unbounded 
+ \<Longrightarrow> hungarian_loop_fail_cond state"
+  by(cases "path_search (buddies state) (potential state)")
+    (auto simp add: hungarian_loop_fail_cond_def)
+
+definition  "hungarian_loop_succ_cond state =
+     (let M = buddies state;
+          \<pi> = potential state in
+       case path_search M \<pi> of
+         Dual_Unbounded \<Rightarrow> False
+       | Lefts_Matched \<Rightarrow> True
+       | Next_Iteration P \<pi>' \<Rightarrow> False)"
+
+lemma hungarian_loop_succ_condE:
+"hungarian_loop_succ_cond state \<Longrightarrow>
+(path_search (buddies state) (potential state) = Lefts_Matched \<Longrightarrow> P)
+ \<Longrightarrow> P"
+and hungarian_loop_succ_condI:
+"path_search (buddies state) (potential state) = Lefts_Matched
+ \<Longrightarrow> hungarian_loop_succ_cond state"
+  by(cases "path_search (buddies state) (potential state)")
+    (auto simp add: hungarian_loop_succ_cond_def)
+
+definition  "hungarian_loop_cont_cond state =
+     (let M = buddies state;
+          \<pi> = potential state in
+       case path_search M \<pi> of
+         Dual_Unbounded \<Rightarrow> False
+       | Lefts_Matched \<Rightarrow> False
+       | Next_Iteration P \<pi>' \<Rightarrow> True)"
+
+lemma hungarian_loop_cont_condE:
+"hungarian_loop_cont_cond state \<Longrightarrow>
+(\<And>p \<pi>'. path_search (buddies state) (potential state) = Next_Iteration p \<pi>' \<Longrightarrow> P)
+ \<Longrightarrow> P"
+and  hungarian_loop_cont_condI:
+" path_search (buddies state) (potential state) = Next_Iteration p \<pi>' \<Longrightarrow> 
+hungarian_loop_cont_cond state"
+  by(cases "path_search (buddies state) (potential state)")
+    (auto simp add: hungarian_loop_cont_cond_def)
+
+lemma hungarian_loop_cases:
+  assumes "hungarian_loop_fail_cond state \<Longrightarrow> P"
+          "hungarian_loop_succ_cond state \<Longrightarrow> P"
+          "hungarian_loop_cont_cond state \<Longrightarrow> P"
+    shows P
+  using assms
+  apply(cases "path_search (buddies state) (potential state)")
+  by(auto simp add: hungarian_loop_fail_cond_def 
+                    hungarian_loop_cont_cond_def
+                    hungarian_loop_succ_cond_def)
+
+lemma hungarian_loop_domintros:
+  "hungarian_loop_fail_cond state \<Longrightarrow> hungarian_loop_dom state"
+  "hungarian_loop_succ_cond state \<Longrightarrow> hungarian_loop_dom state"
+  "\<lbrakk>hungarian_loop_cont_cond state; hungarian_loop_dom (hungarian_loop_upd state)\<rbrakk>
+    \<Longrightarrow> hungarian_loop_dom state"
+    apply(all \<open>rule hungarian_loop.domintros\<close>)
+    apply(all \<open>cases "path_search (buddies state) (potential state)"\<close>)
+    by(auto simp add: hungarian_loop_fail_cond_def 
+                      hungarian_loop_cont_cond_def
+                      hungarian_loop_succ_cond_def
+                      hungarian_loop_upd_def)
+
+lemma hungarian_loop_simps:
+ "hungarian_loop_fail_cond state \<Longrightarrow> hungarian_loop state = hungarian_loop_fail state"
+ "hungarian_loop_succ_cond state \<Longrightarrow> hungarian_loop state = hungarian_loop_succ state"
+ "\<lbrakk>hungarian_loop_cont_cond state; hungarian_loop_dom state\<rbrakk>
+   \<Longrightarrow> hungarian_loop state = hungarian_loop (hungarian_loop_upd state)"
+  by(auto simp add: hungarian_loop.psimps[OF hungarian_loop_domintros(1)] 
+                    hungarian_loop.psimps[OF hungarian_loop_domintros(2)] 
+                    hungarian_loop.psimps  hungarian_loop_upd_def
+                    hungarian_loop_fail_def hungarian_loop_succ_def
+            elim: hungarian_loop_fail_condE hungarian_loop_succ_condE
+                  hungarian_loop_cont_condE)
+
+lemma fail_cond_after_fail_upd:
+  "hungarian_loop_fail_cond state \<Longrightarrow> hungarian_loop_fail_cond (hungarian_loop_fail state)"
+  by(auto elim!: hungarian_loop_fail_condE
+         intro!: hungarian_loop_fail_condI
+       simp add: hungarian_loop_fail_def)
+
+lemma succ_cond_after_succ_upd:
+  "hungarian_loop_succ_cond state \<Longrightarrow> hungarian_loop_succ_cond (hungarian_loop_succ state)"
+  by(auto elim!: hungarian_loop_succ_condE
+         intro!: hungarian_loop_succ_condI
+       simp add: hungarian_loop_succ_def)
+
+lemma succ_and_fail_impossible:
+ "\<lbrakk>hungarian_loop_succ_cond state; hungarian_loop_fail_cond state\<rbrakk>
+ \<Longrightarrow> False"
+  by(auto elim!: hungarian_loop_succ_condE hungarian_loop_fail_condE)
+
+lemma hungarian_loop_induct:
+  assumes "hungarian_loop_dom state"
+           "\<And> state. \<lbrakk>hungarian_loop_dom state;
+                      hungarian_loop_cont_cond state \<Longrightarrow> P (hungarian_loop_upd state)\<rbrakk>
+                     \<Longrightarrow> P state"
+     shows "P state"
+proof(induction rule: hungarian_loop.pinduct[OF assms(1)])
+  case (1 state)
+  note IH = this
+show ?case 
+  proof(cases state rule: hungarian_loop_cases, goal_cases)
+    case 1
+    then show ?case
+     by(auto elim!:  hungarian_loop_fail_condE
+            intro!: assms(2)[OF IH(1)]
+          simp add: hungarian_loop_cont_cond_def)
+  next
+    case 2
+    then show ?case 
+     by(auto elim!:  hungarian_loop_succ_condE
+            intro!: assms(2)[OF IH(1)] 
+          simp add: hungarian_loop_cont_cond_def)
+  next
+    case 3
+    show ?case 
+      apply(rule assms(2)[OF IH(1)])
+      using 3 
+      by(auto intro!: IH(2)
+               elim!: hungarian_loop_cont_condE
+            simp add: hungarian_loop_upd_def Let_def 
+               split: option.split prod.split path_search_result.splits)
+  qed
+qed
+
+lemma flag_unchanged: "result (hungarian_loop_upd state) = result state"
+  by(auto simp add: hungarian_loop_upd_def Let_def)
+
+lemma flag_fail: "result (hungarian_loop_fail state) = failure"
+  by(auto simp add: hungarian_loop_fail_def Let_def)
+
+lemma flag_succ: "result (hungarian_loop_succ state) = success"
+  by(auto simp add: hungarian_loop_succ_def Let_def)
+
+definition "path_search_precond M \<pi> =
+  (matching_invar M \<and> potential_invar \<pi> \<and> graph_matching G (matching_abstract M) \<and>
+  matching_abstract M \<subseteq> tight_subgraph G edge_costs (potential_abstract \<pi>) \<and>
+  feasible_min_perfect_dual G edge_costs (potential_abstract \<pi>))"
+
+lemma path_search_precondI:
+"\<lbrakk>matching_invar M; potential_invar \<pi>;
+  matching_abstract M \<subseteq> tight_subgraph G edge_costs (potential_abstract \<pi>);
+  graph_matching G (matching_abstract M);
+  feasible_min_perfect_dual G edge_costs (potential_abstract \<pi>)\<rbrakk>
+\<Longrightarrow> path_search_precond M \<pi>"
+and path_search_precondE:
+"path_search_precond M \<pi> \<Longrightarrow>
+ (\<lbrakk>matching_invar M; potential_invar \<pi>;
+  matching_abstract M \<subseteq> tight_subgraph G edge_costs (potential_abstract \<pi>);
+  graph_matching G (matching_abstract M);
+  feasible_min_perfect_dual G edge_costs (potential_abstract \<pi>)\<rbrakk> \<Longrightarrow> P)
+\<Longrightarrow> P"
+and path_search_precondD:
+"path_search_precond M \<pi> \<Longrightarrow> matching_invar M"
+"path_search_precond M \<pi> \<Longrightarrow> potential_invar \<pi>"
+"path_search_precond M \<pi> \<Longrightarrow> graph_matching G (matching_abstract M)"
+"path_search_precond M \<pi> \<Longrightarrow> 
+   matching_abstract M \<subseteq> tight_subgraph G edge_costs (potential_abstract \<pi>)"
+"path_search_precond M \<pi> \<Longrightarrow> 
+   feasible_min_perfect_dual G edge_costs (potential_abstract \<pi>)"
+  by(auto simp add: path_search_precond_def)
+
+definition "good_search_result M \<pi>' p =
+        (potential_invar \<pi>' \<and> 
+        matching_abstract M \<subseteq> tight_subgraph G edge_costs (potential_abstract \<pi>') \<and>
+        feasible_min_perfect_dual G edge_costs (potential_abstract \<pi>') \<and> 
+        set (edges_of_path p) \<subseteq> tight_subgraph G edge_costs (potential_abstract \<pi>') \<and>
+        graph_augmenting_path G (matching_abstract M) p)"
+
+lemma good_search_resultE:
+"good_search_result M \<pi>' p \<Longrightarrow>
+ (\<lbrakk>potential_invar \<pi>'; 
+   matching_abstract M \<subseteq> tight_subgraph G edge_costs (potential_abstract \<pi>');
+   feasible_min_perfect_dual G edge_costs (potential_abstract \<pi>'); 
+   set (edges_of_path p) \<subseteq> tight_subgraph G edge_costs (potential_abstract \<pi>');
+   graph_augmenting_path G (matching_abstract M) p\<rbrakk> 
+ \<Longrightarrow> P)
+\<Longrightarrow> P"
+and good_search_resultI:
+"\<lbrakk>potential_invar \<pi>'; 
+   matching_abstract M \<subseteq> tight_subgraph G edge_costs (potential_abstract \<pi>');
+   feasible_min_perfect_dual G edge_costs (potential_abstract \<pi>'); 
+   set (edges_of_path p) \<subseteq> tight_subgraph G edge_costs (potential_abstract \<pi>');
+   graph_augmenting_path G (matching_abstract M) p\<rbrakk> 
+ \<Longrightarrow> good_search_result M \<pi>' p"
+and good_search_resultD:
+"good_search_result M \<pi>' p \<Longrightarrow> potential_invar \<pi>'"
+"good_search_result M \<pi>' p \<Longrightarrow> 
+  matching_abstract M \<subseteq> tight_subgraph G edge_costs (potential_abstract \<pi>')"
+"good_search_result M \<pi>' p \<Longrightarrow> 
+   feasible_min_perfect_dual G edge_costs (potential_abstract \<pi>')"
+"good_search_result M \<pi>' p \<Longrightarrow>
+   set (edges_of_path p) \<subseteq> tight_subgraph G edge_costs (potential_abstract \<pi>')"
+"good_search_result M \<pi>' p \<Longrightarrow> graph_augmenting_path G (matching_abstract M) p"
+  by(auto simp add: good_search_result_def)
+
+end
+
+subsection \<open>Locale for Proofs\<close>
+
+locale hungarian_loop = 
+ hungarian_loop_spec where edge_costs = edge_costs
+for edge_costs::"'v set \<Rightarrow> real" +
+fixes L R
+assumes G: 
+   "bipartite G L R"
+   "card_L = card L"
+   "card_R = card R"
+   "finite L"
+   "finite R"
+   "L \<union> R \<subseteq> Vs G"
+   
+and potential:
+ "potential_invar init_potential"
+ "feasible_min_perfect_dual G edge_costs (potential_abstract init_potential)"
+and matching:
+  "\<And> M. matching_invar M \<Longrightarrow> graph_matching G (matching_abstract M)"
+  "matching_invar empty_matching"
+  "matching_abstract empty_matching = {}"
+and augment:
+  "\<And> M p. \<lbrakk>matching_invar M; graph_augmenting_path G (matching_abstract M) p\<rbrakk> \<Longrightarrow> 
+         matching_invar (augment M p)"
+  "\<And> M p. \<lbrakk>matching_invar M; graph_augmenting_path G (matching_abstract M) p\<rbrakk> \<Longrightarrow> 
+         matching_abstract (augment M p) =  matching_abstract M \<oplus> set (edges_of_path p)"
+and path_search:
+  "\<And> M \<pi> B. \<lbrakk>path_search_precond M \<pi>; path_search M \<pi> = Dual_Unbounded\<rbrakk>
+    \<Longrightarrow> \<exists> \<pi>'. feasible_min_perfect_dual G edge_costs \<pi>' \<and> sum \<pi>' (L \<union> R) > B"
+   "\<And> M \<pi>. \<lbrakk>path_search_precond M \<pi>; path_search M \<pi> = Lefts_Matched\<rbrakk> 
+    \<Longrightarrow> L \<subseteq> Vs (matching_abstract M)"
+   "\<And> M \<pi> \<pi>' p. \<lbrakk>path_search_precond M \<pi>; path_search M \<pi> = Next_Iteration p \<pi>'\<rbrakk> 
+    \<Longrightarrow> good_search_result M \<pi>' p" 
+begin
+
+lemma graph_matching_finite: "graph_matching G M \<Longrightarrow> finite M" 
+  using  finite_Vs_then_finite[of M] finite_parts_bipartite_graph_invar[OF G(4,5,1)]
+      graph_invar_subset
+  by auto
+
+subsection \<open>Invariant Setup\<close>
+
+definition "state_invar state = 
+  (matching_invar (buddies state) \<and> potential_invar (potential state) \<and>
+   graph_matching G (matching_abstract (buddies state)) \<and>
+  matching_abstract (buddies state) \<subseteq> 
+        tight_subgraph G edge_costs (potential_abstract (potential state)) \<and>
+  feasible_min_perfect_dual G edge_costs (potential_abstract (potential state)))"
+
+lemma state_invarE:
+"state_invar state \<Longrightarrow> 
+ (\<lbrakk>matching_invar (buddies state); potential_invar (potential state);
+   graph_matching G (matching_abstract (buddies state));
+  matching_abstract (buddies state) \<subseteq> 
+        tight_subgraph G edge_costs (potential_abstract (potential state));
+  feasible_min_perfect_dual G edge_costs (potential_abstract (potential state))\<rbrakk>
+  \<Longrightarrow> P)
+ \<Longrightarrow> P"
+and state_invarI:
+"\<lbrakk>matching_invar (buddies state); potential_invar (potential state);
+   graph_matching G (matching_abstract (buddies state));
+  matching_abstract (buddies state) \<subseteq> 
+        tight_subgraph G edge_costs (potential_abstract (potential state));
+  feasible_min_perfect_dual G edge_costs (potential_abstract (potential state))\<rbrakk>
+  \<Longrightarrow> state_invar state"
+and state_invarD:
+"state_invar state \<Longrightarrow> matching_invar (buddies state)"
+"state_invar state \<Longrightarrow> potential_invar (potential state)"
+"state_invar state \<Longrightarrow> graph_matching G (matching_abstract (buddies state))"
+"state_invar state \<Longrightarrow> 
+   matching_abstract (buddies state) \<subseteq> 
+        tight_subgraph G edge_costs (potential_abstract (potential state))"
+"state_invar state \<Longrightarrow> 
+  feasible_min_perfect_dual G edge_costs (potential_abstract (potential state))"
+  by(auto simp add: state_invar_def)
+
+subsection \<open>Invariant Preservation\<close>
+
+lemma 
+  assumes "hungarian_loop_cont_cond state"  "state_invar state"
+ shows state_invar_pres_one_step:
+    "state_invar (hungarian_loop_upd state)"
+ and card_increase: "card (matching_abstract (buddies (hungarian_loop_upd state)))
+                     > card (matching_abstract (buddies state))"
+proof-
+  define M where "M = buddies state"
+  define \<pi> where "\<pi> = potential state"
+  obtain p \<pi>' where path_search_result_is:  "path_search M \<pi> = Next_Iteration p \<pi>'"
+    using assms(1)
+    by(auto elim!: hungarian_loop_cont_condE simp add: M_def \<pi>_def)
+  note state_invars = state_invarD[OF assms(2), folded M_def \<pi>_def]
+  hence path_search_precond: "path_search_precond M \<pi>"
+    by(auto intro!: path_search_precondI)
+  note path_search_props = path_search(3)[OF path_search_precond path_search_result_is]
+  note path_search_props_unfolded = 
+         good_search_resultD[OF path_search_props]
+  define M' where "M' = augment M p"
+  have state'_is: "hungarian_loop_upd state = state \<lparr>buddies:=M', potential := \<pi>' \<rparr>"
+    using path_search_result_is
+    by(auto simp add: hungarian_loop_upd_def M'_def M_def \<pi>_def)
+  have matching_invar': "matching_invar M'" 
+    by(auto intro!: augment(1) simp add: M'_def state_invars(1) path_search_props_unfolded(5))
+  have M'_is: "matching_abstract M' = matching_abstract M \<oplus> set (edges_of_path p)"
+    using  state_invars(1) path_search_props_unfolded(5)
+    by(auto simp add: augment(2) M'_def)
+  hence new_matching_valid: "graph_matching G (matching_abstract M')"
+    using  state_invars(1) path_search_props_unfolded(5) state_invars(3)
+    by(auto intro!: graph_matching_finite dest: Berge_2')
+  have M'_tight:
+     "matching_abstract M' \<subseteq> tight_subgraph G edge_costs (potential_abstract \<pi>')" 
+  proof(rule, goal_cases)
+    case (1 e)
+   hence  "e \<in> matching_abstract M \<or> e \<in> set (edges_of_path p)" "e \<in> G" 
+     using state_invars(3) path_search_props_unfolded(5)
+     by(auto simp add: in_symmetric_diff_iff M'_is intro: path_ball_edges )
+   then show ?case 
+     using path_search_props_unfolded(2,4)
+     by auto
+ qed
+    show "state_invar (hungarian_loop_upd state)"
+      using new_matching_valid  M'_tight
+      by(auto intro!: state_invarI matching_invar' path_search_props_unfolded 
+            simp add: state'_is)
+    show  "card (matching_abstract (buddies (hungarian_loop_upd state)))
+                     > card (matching_abstract (buddies state))"
+      by(auto intro!: new_matching_bigger graph_matching_finite state_invars(3)
+            simp add: state'_is M_def[symmetric] M'_is  path_search_props_unfolded(5,1))
+  qed
+
+lemma 
+ assumes "state_invar state"
+ shows state_invar_pres_fail: "state_invar (hungarian_loop_fail state)"
+   and state_invar_pres_succ: "state_invar (hungarian_loop_succ state)"
+  using assms
+  by(auto intro!: state_invarI
+           elim!: state_invarE
+        simp add: hungarian_loop_fail_def hungarian_loop_succ_def)
+
+lemma state_invar_pres:
+  assumes "hungarian_loop_dom state"
+          "state_invar state"
+    shows "state_invar (hungarian_loop state)"
+  using assms(2)
+proof(induction rule: hungarian_loop_induct[OF assms(1)])
+  case (1 state)
+  then show ?case
+    by(cases state rule: hungarian_loop_cases)
+      (auto intro: state_invar_pres_fail state_invar_pres_succ 
+                   state_invar_pres_one_step 
+         simp add: hungarian_loop_simps)
+qed
+
+subsection \<open>Termination\<close>
+
+lemma hungarian_loop_termination_induction:
+  assumes "state_invar state"
+          "n = card G - card (matching_abstract (buddies state))"
+    shows "hungarian_loop_dom state"
+  using assms
+proof(induction n arbitrary: state rule: less_induct)
+  case (less n)
+  show ?case 
+  proof(cases state rule: hungarian_loop_cases)
+    case 3
+    note invar_later = state_invar_pres_one_step[OF 3 less(2)]
+    hence card_later_less_G:
+        "card (matching_abstract (buddies (hungarian_loop_upd state))) \<le> card G"
+      using G(1,4,5)  finite_Vs_then_finite finite_parts_bipartite_graph_invar
+      by(auto intro!: card_mono dest!: state_invarD(3))
+    hence card_decrease:
+         "card G - card (matching_abstract (buddies (hungarian_loop_upd state))) < n"
+      using card_increase[OF 3 less(2)] less(3) by linarith
+    show ?thesis 
+      using 3 less(1) card_decrease invar_later
+      by(auto intro: hungarian_loop_domintros(3))
+  qed (simp_all add: hungarian_loop_domintros(1,2))
+qed
+
+lemmas hungarian_loop_termination = hungarian_loop_termination_induction[OF _ refl]
+
+subsection \<open>Correctness\<close>
+
+lemma final_flag:
+  assumes "hungarian_loop_dom state"
+    shows "result (hungarian_loop state) \<noteq> notyetterm"
+proof(induction rule: hungarian_loop_induct[OF assms(1)])
+  case (1 state)
+  then show ?case
+    by(cases state rule: hungarian_loop_cases)
+      (auto simp add: hungarian_loop_simps flag_fail flag_succ)
+qed
+
+lemma if_fail_flag_then_fail:
+  assumes "hungarian_loop_dom state" "result (hungarian_loop state) = failure"
+  shows "hungarian_loop_fail_cond (hungarian_loop state)"
+  using assms(2)
+proof(induction rule: hungarian_loop_induct[OF assms(1)])
+  case (1 state)
+  then show ?case
+    by(cases state rule: hungarian_loop_cases)
+      (auto simp add: hungarian_loop_simps  hungarian_loop_succ_def
+               intro: fail_cond_after_fail_upd)
+qed
+
+lemma if_succ_flag_then_succ:
+  assumes "hungarian_loop_dom state" "result (hungarian_loop state) = success"
+  shows "hungarian_loop_succ_cond (hungarian_loop state)"
+  using assms(2)
+proof(induction rule: hungarian_loop_induct[OF assms(1)])
+  case (1 state)
+  then show ?case
+    by(cases state rule: hungarian_loop_cases)
+      (auto simp add: hungarian_loop_simps  hungarian_loop_fail_def
+               intro: succ_cond_after_succ_upd)
+qed
+
+lemma min_perfect_if_algo_says_so:
+  assumes "hungarian_loop_succ_cond state"
+          "state_invar state" "card_L = card_R"
+  shows   "min_weight_perfect_matching G edge_costs (matching_abstract (buddies state))"
+proof-
+  have "L \<subseteq> Vs (matching_abstract (buddies state))" 
+    using assms(1,2)
+    by(intro path_search(2))
+      (auto elim!: hungarian_loop_succ_condE state_invarE
+            intro: path_search_precondI)
+  hence perfect: "perfect_matching G (matching_abstract (buddies state))"
+    using  assms(2,3) 
+    by (auto intro: all_left_matched_perfect[OF G(1)] 
+             elim!: state_invarE 
+          simp add: G(2,3,5))
+  thus ?thesis
+    using G(1,4,5) finite_parts_bipartite_graph_invar state_invarD(4,5)[OF assms(2)]
+    by(auto intro!: min_weight_perfect_if_tight(1)[of _ _ "potential_abstract (potential state)"])
+qed
+
+lemma infeasible_if_sides_unequal_size:
+  "card_L \<noteq> card_R \<Longrightarrow> \<nexists> M. perfect_matching G M"
+  using G(6)
+  by(intro no_perfect_matching_one_side_bigger)
+    (auto intro!: G(1) simp add: G(2,3))
+
+lemma no_perfect_if_algo_says_so:
+  assumes "hungarian_loop_fail_cond state"
+          "state_invar state"
+    shows "\<nexists> M. perfect_matching G M"
+proof(rule notI, goal_cases)
+  case 1
+  then obtain M where M: "perfect_matching G M" 
+    by auto
+  define B where "B = sum edge_costs M"
+  obtain \<pi> where pi: "feasible_min_perfect_dual G edge_costs \<pi>" "B < sum \<pi> (L \<union> R)"
+    using assms(1,2)
+    by(auto elim!: hungarian_loop_fail_condE state_invarE 
+            dest!: path_search(1)[OF path_search_precondI])
+  moreover hence "sum \<pi> (Vs G) \<le> sum edge_costs M"
+    using M G(1,4,5) finite_parts_bipartite_graph_invar
+    by(auto intro!: min_perfect_matching_weak_duality)
+  moreover have "L \<union> R = Vs G"
+    using G(1,6) bipartite_vs_subset by blast
+  ultimately show False
+    by(auto simp add: B_def)
+qed
+
+subsection \<open>The Initial State\<close>
+
+lemma initial_state_invar: 
+  "state_invar initial_state"
+  by(auto intro!: state_invarI 
+        simp add: initial_state_def matching potential)
+
+lemma initial_state_hungarian_dom:
+  "hungarian_loop_dom initial_state"
+  by (simp add: hungarian_loop_termination initial_state_invar)
+
+lemma initial_state_loops_same:
+  "hungarian_loop_impl initial_state = hungarian_loop initial_state"
+  by (simp add: hungarian_loop_impl_same initial_state_hungarian_dom)
+
+lemma loop_on_initial_state_invar:
+  "state_invar (hungarian_loop initial_state)"
+  by (simp add: initial_state_hungarian_dom initial_state_invar state_invar_pres)
+
+subsection \<open>Final Correctness\<close>
+
+theorem hungarian_correctness:
+ "hungarian = None \<Longrightarrow> \<nexists> M. perfect_matching G M"
+ "hungarian = Some M \<Longrightarrow> min_weight_perfect_matching G edge_costs (matching_abstract M)"
+proof(goal_cases)
+  case 1
+  show ?case
+  proof(cases "card_L = card_R")
+    case True
+    hence "result (hungarian_loop initial_state) = failure" 
+      using 1 initial_state_hungarian_dom 
+      by(auto simp add: Let_def result.split[of "\<lambda> x. x = None"]
+                        initial_state_loops_same if_split[of "\<lambda> x. x = None"]
+                        hungarian_loop_spec.hungarian_def
+                 intro: result.exhaust[of "result (hungarian_loop initial_state)"]
+                  dest: final_flag) 
+    hence "hungarian_loop_fail_cond (hungarian_loop initial_state)" 
+      using if_fail_flag_then_fail initial_state_hungarian_dom by blast
+    then show ?thesis 
+      using loop_on_initial_state_invar
+      by(rule no_perfect_if_algo_says_so)
+  next
+    case False
+    then show ?thesis 
+      by(rule infeasible_if_sides_unequal_size)
+  qed
+next
+  case 2
+  hence "result (hungarian_loop initial_state) = success" 
+      and same_cards:"card_L = card_R"
+      and M_is: "M = buddies (hungarian_loop initial_state)"
+      using 2 initial_state_hungarian_dom
+      by(auto simp add: hungarian_def Let_def result.split[of "\<lambda> x. x = Some _"]
+                        if_split[of "\<lambda> x. x = Some _"] initial_state_loops_same 
+                 intro: result.exhaust[of "result (hungarian_loop initial_state)"]
+                  dest: final_flag) 
+    hence "hungarian_loop_succ_cond (hungarian_loop initial_state)" 
+      using if_succ_flag_then_succ initial_state_hungarian_dom by blast
+    thus ?case
+      using loop_on_initial_state_invar same_cards
+      by(auto intro!: min_perfect_if_algo_says_so simp add: M_is)
+  qed
+
+end
+end
